\subsection{CS Mathematics Handbook}Extracts from \cite{MathHbk:05}, which themselvesare taken from the rear of \cite{gries.93}.\subsubsection{Theorems of the Propositional Calculus}\textsc{Equivalence and \textit{true}\\}\begin{tabular}{ll}(3.1) & Axiom, Associativity of $\equiv$ : $((p\equiv q)\equiv r) \equiv (p\equiv (q\equiv r))$\\(3.2) & Axiom, Symmetry of  $\equiv$ : $p\equiv q\equiv q \equiv p$\\(3.3) & Axiom, Identity of  $\equiv$ : $\mbox{\textit{true}} \equiv q\equiv q $\\(3.4) & $\mbox{\textit{true}}$\\(3.5) & Reflexivity of  $\equiv$ : $p\equiv p $\\\end{tabular}\ \par\textsc{Negation, inequivalence and \textit{false}\\}\begin{tabular}{ll}(3.8) & Axiom, Definition of \textit{false} : $\mbox{\textit{false}} \equiv \neg \mbox{\textit{true}}$\\(3.9) & Axiom, Distributivity of  $\neg$ over $\equiv$ : $\neg(p\equiv q) \equiv \neg p \equiv q$\\(3.10) & Axiom, Definition of $\not \equiv$ : $(p\not\equiv q) \equiv \neg(p\equiv q)$\\(3.11) & $\neg p\equiv q \equiv p \equiv \neg q$\\(3.12) &  Double negation : $\neg \neg p \equiv p$\\(3.13) &  Negation of \textit{false} : $\neg \mbox{\textit{false}} \equiv \mbox{\textit{true}}$\\(3.14) &  $(p\not \equiv q) \equiv \neg p \equiv q$\\(3.15) &  $\neg p \equiv p \equiv \mbox{\textit{false}}$\\(3.16) &  Symmetry of $\not \equiv$ : $(p\not \equiv q) \equiv (q\not\equiv p)$\\(3.17) &  Associativity of $\not\equiv$ : $((p\not\equiv q)\not\equiv r) \equiv (p\not\equiv (q\not\equiv r))$\\(3.18) &  Mutual associativity : $((p\not \equiv q)\equiv r) \equiv (p\not\equiv (q\equiv r))$\\(3.19) &  Mutual Interchangeability : $p\not \equiv q \equiv r\ \equiv\ p\equiv q\not \equiv r$\\\end{tabular}\ \par\textsc{Disjunction\\}\begin{tabular}{ll}(3.24) & Axiom, Symmetry of $\vee$ : $p\vee q \equiv  q \vee p$\\(3.25) & Axiom, Associativity of  $\vee$  : $ (p\vee q) \vee r \equiv  p \vee (q \vee r)$\\(3.26) & Axiom, Idempotency of $\vee$ : $p\vee p \equiv p$\\(3.27) & Axiom, Distributivity of $\vee$ over $\equiv$ : $p \vee (q\equiv r) \equiv p\vee q \equiv p \vee r$\\(3.28) & Axiom,  Excluded Middle : $p \vee \neg p $\\(3.29) &  Zero of $\vee$ : $p \vee \mbox{\textit{true}} \equiv \mbox{\textit{true}}$\\(3.30) &  Identity of $\vee$ : $p\vee \mbox{\textit{false}} \equiv  p$\\(3.31) &  Distributivity of $\vee$ over $\vee$ : $p \vee (q\vee r) \equiv (p\vee q) \vee (p \vee r)$\\(3.32) &  $p\vee q \equiv p \vee \neg q \equiv p $\\\end{tabular}\ \par\textsc{Conjunction\\}\begin{tabular}{lll}(3.35) & Axiom, Golden rule : $p\wedge q \equiv  p \equiv q \equiv p \vee q$\\(3.36) & Symmetry of  $\wedge$  : $ p\wedge q \equiv  q \wedge p$\\(3.37) & Associativity of  $\wedge$  : $ (p\wedge q) \wedge r \equiv  p \wedge (q \wedge r)$\\(3.38) & Idempotency of $\wedge$ : $p\wedge p \equiv p$\\(3.39) & Identity of $\wedge$ : $p\wedge \mbox{\textit{true}} \equiv  p$\\(3.40) & Zero of $\wedge$ : $p \wedge \mbox{\textit{false}} \equiv \mbox{\textit{false}}$\\(3.41) & Distributivity of $\wedge$ over $\wedge$ : $p \wedge (q\wedge r) \equiv (p\wedge q) \wedge (p \wedge r)$\\(3.42) & Contradiction : $p \wedge \neg p \equiv \mbox{\textit{false}}$\\\end{tabular}\begin{tabular}{lll}(3.43) & Absortion: & (a) $p\wedge (p\vee q) \equiv p$\\	& 	    & (b) $p \vee (p \wedge q) \equiv p$\\(3.44) & Absortion: & (a) $p \wedge (\neg p\vee q) \equiv p \wedge  q$\\	&	    & (b) $p \vee (\neg p \wedge q) \equiv p \vee q$\\\end{tabular}\begin{tabular}{lll}(3.45) &  Distributivity of $\vee$ over $\wedge$ : $p \vee (q\wedge r) \equiv (p\vee q) \wedge (p \vee r)$\\(3.46) & Distributivity of $\wedge$ over $\vee$ : $p \wedge (q\vee r) \equiv (p\wedge q) \vee (p \wedge r)$\\\end{tabular}\begin{tabular}{lll}(3.47) &  De Morgan: & (a) $\neg (p\wedge q) \equiv \neg p \vee \neg q  $\\       &  	     & (b) $\neg (p\vee q) \equiv \neg p \wedge \neg q $\\\end{tabular}\begin{tabular}{lll}(3.48) &  $p\wedge q \equiv p \wedge \neg q \equiv \neg p $\\(3.49) &  $p\wedge (q \equiv r) \equiv p\wedge q \equiv p\wedge r \equiv p $\\(3.50) &  $p\wedge (q \equiv p) \equiv p \wedge q  $\\(3.51) &  Replacement : $ (p\equiv q) \wedge (r \equiv p) \equiv (p\equiv q) \wedge (r\wedge q) $\\(3.52) &  Definition of $\equiv$ : $ p \equiv q \equiv (p\wedge q) \vee (\neg p \wedge \neg q) $\\(3.53) &  Exclusive or : $p\not \equiv q \equiv (\neg p \wedge q) \vee (p\wedge \neg q) $\\(3.55) &  $(p\wedge q) \wedge r \equiv p \equiv q \equiv r \equiv p\vee q \equiv q\vee r \equiv r \vee p \equiv p \vee q \vee r $\\\end{tabular}\ \par\textsc{Implication\\}\begin{tabular}{lll}(3.57) & Axiom, Definition of Implication: $ p\Rightarrow q \equiv p\vee  q \equiv q $\\(3.58) & Axiom, Consequence : $p\Leftarrow q \equiv q\Rightarrowp$\\(3.59) & Definition of implication : $ p\Rightarrow q \equiv\neg p\vee  q $\\(3.60) & Definition of implication : $p\Rightarrow q \equiv p\wedge  q\equiv p $\\ (3.61) &Contrapositive : $  p\Rightarrow q \equiv \neg q\Rightarrow  \negp $\\ (3.62) & $p\Rightarrow (q\equiv r) \equiv p\wedge q \equiv p\wedge r$\\ (3.63) & Distributivity of $\Rightarrow$ over $\equiv$: $p \Rightarrow (q\equiv r) \equiv p\Rightarrow q \equiv p\Rightarrow r$\\ (3.64) &  $p \Rightarrow (q\equiv r) \equiv(p\Rightarrow q) \Rightarrow (p \Rightarrow r)$\\ (3.65) &Shunting : $p \wedge q\Rightarrow r \equiv p\Rightarrow (q\Rightarrow r)$\\ (3.66) &  $p \wedge (p\Rightarrow q) \equiv p\wedge q$\\ (3.67) &  $p \wedge (q\Rightarrow p) \equiv p$\\ (3.68) &  $p \vee (p\Rightarrow q) \equiv \mbox{\textit{true}}$\\ (3.69) &  $p \vee (q\Rightarrow p) \equiv q\Rightarrow p$\\(3.70) &  $p \vee q\Rightarrow p\wedge q \equiv p \equiv q$\\(3.71) & Reflexivity of $\Rightarrow$ : $p\Rightarrow p \equiv \mbox{\textit{true}}$\\(3.72) & Right zero of $\Rightarrow$ : $p \Rightarrow \mbox{\textit{true}} \equiv \mbox{\textit{true}}$\\(3.73) & Left identity of $\Rightarrow$ : $\mbox{\textit{true}} \Rightarrow p \equiv p$\\(3.74) & $p\Rightarrow \mbox{\textit{false}} \equiv \neg p$\\(3.75) & $\mbox{\textit{false}} \Rightarrow p \equiv \mbox{\textit{true}}$\\\end{tabular}\begin{tabular}{lll}(3.76) & Weakening/strengthening : & (a) $ p\Rightarrow p\vee q$\\       & & (b) $ p\wedge q\Rightarrow p$\\       & & (c) $ p\wedge q \Rightarrow p\vee q$\\       & & (d) $ p\vee (q\wedge r) \Rightarrow p\vee q$\\       & & (e) $ p\wedge q \Rightarrow p \wedge (q\vee r)$\\\end{tabular}\begin{tabular}{lll}(3.77) & Modus ponens : $p\wedge (p\Rightarrow q) \Rightarrow q$\\(3.78) & $(p\Rightarrow r)\wedge (q\Rightarrow r) \equiv (p\vee q\Rightarrow r)$\\(3.79) & $(p\Rightarrow r)\wedge (\neg p \Rightarrow r) \equiv r$\\(3.80) & Mutual implication : $(p\Rightarrow q)\wedge (q \Rightarrow p) \equiv (p\equiv q)$\\(3.81) & Antisymmetry : $(p\Rightarrow q)\wedge (q \Rightarrow p) \Rightarrow (p\equiv q)$\\\end{tabular}\begin{tabular}{lll}(3.82) & Transitivity : & (a) $(p\Rightarrow q)\wedge (q \Rightarrow r) \Rightarrow (p\Rightarrow r)$\\       & & (b) $(p\equiv q)\wedge (q \Rightarrow r) \Rightarrow (p\Rightarrow r)$\\       & & (c) $(p\Rightarrow q)\wedge (q \equiv r) \Rightarrow (p\Rightarrow r)$\\\end{tabular}\ \par\subsubsection{Theorems of the Propositional Calculus}The following section is not in \cite{MathHbk:05},and is an specialisation of material at the rear of \cite{gries.93}to address predicates only.\textsc{Laws of Universal Quantification}\begin{tabular}{lll}   (8.13') & Axiom, Empty Range :           &  $(\land x | false : P) = true$\\ (8.14') & Axiom, One-point rule :           &  $(\land x | x=E : P) = P[x:=E], \quad x \notin E$\\ (8.15') & Axiom, Distributivity :           & $(\land x | R : P)\land(\land x | R : Q) = (\land x | R : P \land Q)$\end{tabular} 