\subsection{\textbf{WS} (Owe 1993)}

\def\F{\textsc{f}}
\def\T{\textsc{t}}
\def\pre#1{\textsf{pre-}\!#1}

This is the WS logic of Olaf Owe \cite{Owe93}.

\subsubsection{Definedness}

Definition of $\Delta$:
\begin{eqnarray*}
   \Delta(\bot)         &==& \F
\\ \Delta(\T)           &==& \T
\\ \Delta(\F)           &==& \T
\\ \Delta(x)            &==& \T
\\ \Delta(\lnot a)      &==& \Delta a
\\ \Delta(a \land b)    &==& \Delta(a,b)
                        \lor (\Delta a \land \lnot a)
                        \lor (\Delta b \land \lnot b)
\\ \Delta(a \lor b)     &==& \Delta(a,b)
                        \lor (\Delta a \land a)
                        \lor (\Delta b \land b)
\\ \Delta(a \implies b) &==& \Delta(a,b)
                        \lor (\Delta a \land \lnot a)
                        \lor (\Delta b \land b)
\\ \Delta(\forall x.a)  &==& (\forall x.\Delta a)
                        \lor (\exists x.\Delta a \land \lnot a)
\\ \Delta(\exists x.a)  &==& (\forall x.\Delta a)
                        \lor (\exists x.\Delta a \land a)
\\ \Delta(f(e))         &==& \Delta e \land \pre f (e)
\\ \Delta(e_1=e_2)      &==& \Delta(e_1,e_2)
\\ \Delta(\IF a \THEN e_1 \ELSE e_2)
   &==&
   \Delta a \land (\IF a \THEN \Delta e_1 \ELSE \Delta e_2)
\end{eqnarray*}
Properties of $\Delta$:
\begin{eqnarray*}
   \Delta(\Delta a) && holds
\\ \Delta(\Delta a \land a) && holds
\\ \Delta(\Delta a \implies a) && holds
\\ \Delta(a \implies b)\land(a \implies b)
   &==&
   (\Delta a \implies a) \implies (\Delta b \land b)
\\ \Delta(\forall x.a) \land (\forall x.a)
   &==&
   (\forall x.\Delta a \land a)
\\ \Delta(\forall x.a) \implies (\forall x.a)
   &==&
   (\forall x.\Delta a \implies a)
\\ \Delta(\exists x.a) \land (\exists x.a)
   &==&
   (\exists x.\Delta a \land a)
\\ \Delta(\exists x.a) \implies (\exists x.a)
   &==&
   (\exists x.\Delta a \implies a)
\\ \Delta(a[x:=e]) &whenever& \Delta(a,e)
\\ e_1 == e_2
   &becomes&
   \lnot\Delta e_1 \land \lnot\Delta e_2
   \lor
   \Delta(e_1,e_2) \land e_1 = e_2
\end{eqnarray*}

\newpage
\subsubsection{Inference Rules}

$A \infer c$ is equivalent to $\infer c, \overline A$,
where $,$ denotes $\lor$,
and $\overline{\setof{A_1,\ldots,A_n}}$
is $\setof{\lnot A_1, \ldots, \lnot A_n}$.


$$\begin{array}{c@{\quad}l@{\qquad\qquad}r}
  \INFER{\infer A}{\infer B}, & A \subseteq B & (enrichment)
\\
\\\INFER%
    {\infer A \\ \infer \Delta t}%
    {\infer A[x:=t]}
    && (weak~substitution)
\end{array}$$
Convention from now on:
$$
 \INFER{\ldots \\ \infer A_i \\ \ldots}%
       {\infer A}
       , \quad i \in 1\ldots n
$$
is short for
$$
 \INFER{\ldots \\ \infer A_i,B_i \\ \ldots}%
       {\infer A, \bigcup_{i \in 1 \ldots n} B_i}
$$

$$\begin{array}{c@{\quad}l@{\qquad\qquad}r}
  \BINFER{\infer a,b}{\infer a \lor b} && (\lor)
\\
\\\BINFER{\infer a \\\\ \infer b}{\infer a \land b} && (\land)
\\
\\\BINFER{\infer \lnot a,b}{\infer a \implies b} && (\implies)
\\
\\\BINFER{\infer a \\\\ \infer \lnot a}{\infer \F} && (\lnot)
\\
\\\BINFER{\infer \F,a}{\infer a} && (\F)
\\
\\\BINFER{\infer a,\lnot a}{\infer \Delta a} && (\Delta)
\\
\\\BINFER{\infer a}{\infer \forall x.a} && \mbox{no implicit clause with $x$ free when used forwards}
\\
\\\INFER{\infer \exists x . a \\\\ \infer \lnot a}%
        {\infer \F}
        && \mbox{no implicit clause with $x$ free}
\\
\\\INFER{\infer a[x:=t]}{\infer \exists x.a} && (\exists\mbox{-introduction})
\end{array}$$
\newpage
Logical axioms:
\begin{eqnarray*}
  && \infer a,\lnot a,\lnot\Delta a
\\&& \infer \Delta\Delta t
\end{eqnarray*}
Derived Rules and Theorems:
$$\begin{array}{lrr}
   \BINFER%
     {\infer a}%
     {\infer \Delta a \land a}
   &&
   \BINFER%
     {\infer a \land b}%
     {\infer (\Delta a \land a) \land (\Delta a \land a)}
\\ \\
   \BINFER%
     {\infer \forall x.a}%
     {\infer \forall x.(\Delta a \land a)}
   &&
   \BINFER%
     {\infer a \lor b}%
     {\infer (\Delta a \land a) \lor (\Delta a \land a}
\\ \\
   \BINFER%
     {\infer \exists x.a}%
     {\infer \exists x.(\Delta a \land a)}
   &&
   \BINFER%
     {\infer a \implies b}%
     {\infer (\Delta a \implies a) \implies (\Delta b \land b)}
\\ \\
   \infer \Delta(\Delta a \land a)
   &
   \infer \Delta(\Delta a \implies a)
   &
   \infer \Delta t, \lnot \Delta t
\\ \\
   \INFER%
     {\infer A \\\\ \infer \Delta A[x:=t]}%
     {\infer A[x:=t]}
   && A \mbox{ monotonic, no impicit clause}
\end{array}$$

\subsubsection{Equality}

$$\begin{array}{lrr}
   \infer x=x
   &
   \INFER%
     {\infer e_1 = e_2 \\ \infer a[x:=e_1]}%
     {\infer a[x:=e_2]}
   &
   \BINFER%
     {\infer a \implies b \\\\ \infer b \implies a}%
     {\infer a=b}
\end{array}$$
With strong equality then properties of $\Delta$ above become axioms
and
$$
  \INFER%
    {\infer e_1 == e_2 \\\\ \infer a[x:=e_1]}%
    {\infer a[x:=e_2]}
$$

\subsubsection{Assumptions}

\begin{eqnarray*}
   \BINFER%
     {A \infer a,B}%
     {A,\lnot a \infer B}
   &
   (swap)
   &
   \BINFER%
     {A \infer \lnot a, B}%
     {A,a \infer B}%
\end{eqnarray*}
Derived rules:
$$\begin{array}{c@{\qquad}c@{\qquad}c}
   \BINFER%
     {\infer \Delta a}%
     {a \infer a}
   &
   \BINFER%
     {a \infer b}%
     {\infer a \implies b}
   &
   \INFER%
     {\infer a \\\\ \Delta a,a \infer b}%
     {\infer b}
\end{array}$$


\subsubsection{Function Definitions}

Given $f(y) \defs e$, we have:

$$\begin{array}{c@{\quad}l@{\qquad\qquad}r}
   \infer f(y) == e && (f\mbox{-axiom})
\\ \pre f(y) == \Delta e && (\pre f\mbox{-axiom})
\end{array}$$
If $e$ has recursive calls $f(e_i)$, and $a$ has no occurrence for $f$
and is admissible for $x$,
then:
$$\begin{array}{c@{\quad}l@{\qquad\qquad}r}
   \INFER%
     {\infer a[x:=\bot]
      \\\\
      \ldots,a[x:=f(y)][y:=e_i],\ldots \infer a[x:=e]
      }
     {\infer a[x:=f(y)]}
   && (comp. ind.)
\\ \\
  \INFER%
    {\ldots,\pre f(e_i) \implies a[x:=f(y)][y:=e_i],\ldots
     \infer
     \Delta e \implies a[x:=e]}
    {\pre f(y) \infer a[x:=f(y)]}
    && (\pre f\mbox{-rule})
\end{array}$$


\subsubsection{Propositional Connectives}


\subsubsection{Axioms}


\subsubsection{Inference Rules}


\subsubsection{Derived Rules}


\subsubsection{Valuations}


\subsubsection{Meta-theorems}

