\section{Displaying UTP2LogicDefs}


\verb"\DEFOEESUBST"
\DEFOEESUBST

\newpage
\verb"$$\DEFOEPSUBST{xxx}$$"
$$\DEFOEPSUBST{xxx}$$


\verb"\DEFEEESUBST"
\DEFEEESUBST

\verb"\DEFPPESUBST"
\DEFPPESUBST


\newpage
\verb"$$\DEFEEPSUBST{xxx}$$"
$$\DEFEEPSUBST{xxx}$$


\newpage
\verb"$$\DEFPPPSUBST{xxx}$$"
$$\DEFPPPSUBST{xxx}$$

%\def\AXeqvAssocL{(P\equiv Q)\equiv R}
%\def\AXeqvAssocR{P\equiv (Q\equiv R)}
%\def\AXeqvAssoc{(\AXeqvAssocL) \equiv (\AXeqvAssocR)}
%\def\AXeqvAssocN{\LNAME{Ax-$\equiv$-assoc}}
%
%\def\AXeqvSymm{P\equiv Q\equiv Q \equiv P}
%\def\AXeqvSymmN{\LNAME{Ax-$\equiv$-symm}}
%
%\def\AXeqvId{\textit{true} \equiv Q\equiv Q}
%\def\AXeqvIdN{\LNAME{Ax-$\equiv$-id}}
%
%\def\AXfalseDef{\textit{false} \equiv \neg \mbox{\textit{true}}}
%\def\AXfalseDefN{\LNAME{Ax-$false$-def}}
%
%\def\AXnotEqvDistr{\neg(P\equiv Q) \equiv \neg P \equiv Q}
%\def\AXnotEqvDistrN{\LNAME{Ax-$\neg$-$\equiv$-distr}}
%
%\def\AXorSymm{P\vee Q \equiv  Q \vee P}
%\def\AXorSymmN{\LNAME{Ax-$\vee$-symm}}
%
%\def\AXorAssoc{(P\vee Q) \vee R \equiv  P \vee (Q \vee R)}
%\def\AXorAssocN{\LNAME{Ax-$\vee$-assoc}}
%
%\def\AXorIdem{P\vee P \equiv P}
%\def\AXorIdemN{\LNAME{Ax-$\vee$-idem}}
%
%\def\AXorEqvDistr{P \vee (Q\equiv R) \equiv P\vee Q \equiv P \vee R}
%\def\AXorEqvDistrN{\LNAME{Ax-$\vee$-$\equiv$-distr}}
%
%\def\AXexclMdl{P \vee \neg P}
%\def\AXexclMdlN{\LNAME{Ax-Excl-Mdl}}
%
%\def\AXgoldRule{P\wedge Q \equiv  P \equiv Q \equiv P \vee Q}
%\def\AXgoldRuleN{\LNAME{Ax-Golden-Rule}}
%
%\def\AXimplDef{P\Rightarrow Q \equiv P\vee  Q \equiv Q}
%\def\AXimplDefN{\LNAME{Ax-$\implies$-def}}

\newpage
\verb"$$\AXPROP$$"
$$\AXPROP$$

%\def\AXorAllOScopeL{p \lor (\forall \qsep xs,ys @ q)}
%\def\AXorAllOScopeR{\forall \qsep xs @ p \lor (\forall \qsep ys @ q)}
%\def\AXorAllOScopeS{xs \notin p}
%\def\AXorAllOScopeN{\LNAME{Ax-$\lor$-$\forall x$-scope}}
%\def\AXorAllOScope{\AXorAllOScopeL \equiv \AXorAllOScopeR, \quad \AXorAllOScopeS}
%
%\def\AXorAllEScopeL{p \lor (\forall \qsep Es, Fs @ q)}
%\def\AXorAllEScopeR{\forall \qsep Es @ p \lor (\forall \qsep Fs @ q)}
%\def\AXorAllEScopeS{Es \notin p}
%\def\AXorAllEScopeN{\LNAME{Ax-$\lor$-$\forall E$-scope}}
%\def\AXorAllEScope{\AXorAllEScopeL \equiv \AXorAllEScopeR, \quad \AXorAllEScopeS}
%
%\def\AXorAllPScopeL{p \lor (\forall \qsep Ps,  Qs @ q)}
%\def\AXorAllPScopeR{\forall \qsep Ps @ p \lor (\forall \qsep Qs @ q)}
%\def\AXorAllPScopeS{ Ps \notin p}
%\def\AXorAllPScopeN{\LNAME{Ax-$\lor$-$\forall P$-scope}}
%\def\AXorAllPScope{\AXorAllPScopeL \equiv \AXorAllPScopeR, \quad \AXorAllPScopeS}
%
%\def\AXallODistrL{(\forall \qsep xs @ p \land q)}
%\def\AXallODistrR{(\forall \qsep xs @ p) \land (\forall \qsep xs @ q)}
%\def\AXallODistrN{\LNAME{Ax-$\forall x$-distr}}
%\def\AXallODistr{\AXallODistrL \equiv \AXallODistrR}
%
%\def\AXallEDistrL{(\forall \qsep Es @ p \land q)}
%\def\AXallEDistrR{(\forall \qsep Es @ p) \land (\forall \qsep Es @ q)}
%\def\AXallEDistrN{\LNAME{Ax-$\forall E$-distr}}
%\def\AXallEDistr{\AXallEDistrL \equiv \AXallEDistrR}
%
%\def\AXallPDistrL{(\forall \qsep Ps @ p \land q)}
%\def\AXallPDistrR{(\forall \qsep Ps @ p) \land (\forall \qsep Ps @ q)}
%\def\AXallPDistrN{\LNAME{Ax-$\forall P$-distr}}
%\def\AXallPDistr{\AXallPDistrL \equiv \AXallPDistrR}
%
%\def\AXallOInstL{\forall x\qsep xs @ p}
%\def\AXallOInstR{\forall \qsep xs  @ p[e/x]}
%\def\AXallOInstN{\LNAME{Ax-$\forall x$-inst}}
%\def\AXallOInst{(\AXallOInstL) \implies (\AXallOInstR)}
%
%\def\AXallEInstL{\forall E \qsep Es @ p}
%\def\AXallEInstR{\forall \qsep Es @ p[e/E]}
%\def\AXallEInstN{\LNAME{Ax-$\forall E$-inst}}
%\def\AXallEInst{(\AXallEInstL) \implies (\AXallEInstR)}
%
%\def\AXallPInstL{\forall P\qsep Ps @ p}
%\def\AXallPInstR{\forall \qsep Ps @ p[q/P]}
%\def\AXallPInstN{\LNAME{Ax-$\forall P$-inst}}
%\def\AXallPInst{(\AXallPInstL) \implies (\AXallPInstR)}
%
%\def\AXallORngL{\forall \qsep xs | r @ p}
%\def\AXallORngR{\forall \qsep xs @ r \implies p}
%\def\AXallORngN{\LNAME{Ax-$\forall x$-range}}
%\def\AXallORng{(\AXallORngL) \equiv (\AXallORngR)}
%
%\def\AXanyODefL{\exists \qsep xs @ p}
%\def\AXanyODefR{\lnot (\forall \qsep xs @ \lnot p)}
%\def\AXanyODefN{\LNAME{Ax-$\exists x$-def}}
%\def\AXanyODef{(\AXanyODefL) \equiv \AXanyODefR}
%
%\def\AXanyEDefL{\exists \qsep Es @ p}
%\def\AXanyEDefR{\lnot (\forall \qsep Es @ \lnot p)}
%\def\AXanyEDefN{\LNAME{Ax-$\exists E$-def}}
%\def\AXanyEDef{(\AXanyEDefL) \equiv \AXanyEDefR}
%
%\def\AXanyPDefL{\exists \qsep Ps @ p}
%\def\AXanyPDefR{\lnot (\forall \qsep Ps @ \lnot p)}
%\def\AXanyPDefN{\LNAME{Ax-$\exists P$-def}}
%\def\AXanyPDef{(\AXanyPDefL) \equiv \AXanyPDefR}
%
%\def\AXanyORngL{\exists \qsep xs | r @ p}
%\def\AXanyORngR{\exists \qsep xs @ r \land p}
%\def\AXanyORngN{\LNAME{Ax-$\exists x$-range}}
%\def\AXanyORng{(\AXanyORngL) \equiv (\AXanyORngR)}
%
%\def\AXoneODefL{\exists! \qsep xs @ p}
%\def\AXoneODefR{(\exists \qsep xs @ p)
%                 \land
%                 \exists \qsep ys @ p[ys/\qsep xs] \implies ys = xs}
%\def\AXoneODefN{\LNAME{Ax-$\exists! x$-def}}
%\def\AXoneODef{(\AXoneODefL) \equiv (\AXoneODefR)}
%
%\def\AXoneORngL{\exists! \qsep xs | r @ p}
%\def\AXoneORngR{\exists! \qsep xs @ r \land p}
%\def\AXoneORngN{\LNAME{Ax-$\exists! x$-range}}
%\def\AXoneORng{(\AXoneORngL) \equiv (\AXoneORngR)}
%
%\def\AXeqReflL{e}
%\def\AXeqReflR{e}
%\def\AXeqReflN{\LNAME{Ax-$=$-refl}}
%\def\AXeqRefl{\AXeqReflL = \AXeqReflR}
%
%\def\AXtheDefL{e=\theta x @ p}
%\def\AXtheDefR{p[e/x] \land (\forall y @ p[y/x] \implies y=e)}
%\def\AXtheDefS{x \notin e}
%\def\AXtheDefN{\LNAME{Ax-$\theta$-Def}}
%\def\AXtheDef{(\AXtheDefL) \equiv \AXtheDefR, \quad \AXtheDefS}
%
%\def\AXtheRngL{\theta x | r @ p}
%\def\AXtheRngR{\theta x @ r \land p}
%\def\AXtheRngN{\LNAME{Ax-$\theta$-range}}
%\def\AXtheRng{(\AXtheRngL) = (\AXtheRngR)}
%
%\def\AXObetaRedL{(\lambda x\qsep xs @ e)f}
%\def\AXObetaRedR{(\lambda \qsep xs @ e)[f/x]}
%\def\AXObetaRedN{\LNAME{Ax-$\beta$-OReduce}}
%\def\AXObetaRed{\AXObetaRedL = \AXObetaRedR}
%
%\def\AXEbetaRedL{(\Lambda E\qsep Es @ q)e}
%\def\AXEbetaRedR{(\Lambda \qsep Es @ q)[e/E]}
%\def\AXEbetaRedN{\LNAME{Ax-$\beta$-EReduce}}
%\def\AXEbetaRed{\AXEbetaRedL \equiv \AXEbetaRedR}
%
%\def\AXPbetaRedL{(\Lambda P\qsep Ps @ q)r}
%\def\AXPbetaRedR{(\Lambda \qsep Ps @ q)[r/P]}
%\def\AXPbetaRedN{\LNAME{Ax-$\beta$-PReduce}}
%\def\AXPbetaRed{\AXPbetaRedL \equiv \AXPbetaRedR}
%
%\def\AXLeibnizL{\bigwedge_{i=1}^n x_i = e_i}
%\def\AXLeibnizR{p \equiv p[\vec e/\vec x]}
%\def\AXLeibnizS{x_i \mbox{ distinct}}
%\def\AXLeibnizN{\LNAME{Ax-Leibniz}}
%\def\AXLeibniz{(\AXLeibnizL) \implies (\AXLeibnizR), \quad \AXLeibnizS}
%
%\def\AXOSubstR{p[\vec e/\vec x]}
%\def\AXOSubstL{p[\vec x:=\vec e]}
%\def\AXOSubstN{\LNAME{Ax-OSubst}}
%\def\AXOSubst{\AXOSubstL \equiv \AXOSubstR}
%
%\def\AXESubstL{p[\vec e/Es]}
%\def\AXESubstR{p[Es:=\vec e]}
%\def\AXESubstN{\LNAME{Ax-ESubst}}
%\def\AXESubst{\AXESubstL \equiv \AXESubstR}
%
%\def\AXPSubstL{p[\vec q/ Ps]}
%\def\AXPSubstR{p[ Ps:=\vec q]}
%\def\AXPSubstN{\LNAME{Ax-PSubst}}
%\def\AXPSubst{\AXPSubstL \equiv \AXPSubstR}
%
%\def\AXTrueOSubL{true[\vec e/ \vec x]}
%\def\AXTrueOSubR{true}
%\def\AXTrueOSubN{\LNAME{Ax-$true$-OSubst}}
%\def\AXTrueOSub{\AXTrueOSubL \equiv \AXTrueOSubR}
%
%\def\AXTrueESubL{true[\vec e/ Es]}
%\def\AXTrueESubR{true}
%\def\AXTrueESubN{\LNAME{Ax-$true$-ESubst}}
%\def\AXTrueESub{\AXTrueESubL \equiv \AXTrueESubR}
%
%\def\AXTruePSubL{true[\vec q/ Ps]}
%\def\AXTruePSubR{true}
%\def\AXTruePSubN{\LNAME{Ax-$true$-PSubst}}
%\def\AXTruePSub{\AXTruePSubL \equiv \AXTruePSubR}
%
%\def\AXFalseOSubL{false[\vec e/ \vec x]}
%\def\AXFalseOSubR{false}
%\def\AXFalseOSubN{\LNAME{Ax-$false$-OSubst}}
%\def\AXFalseOSub{\AXFalseOSubL \equiv \AXFalseOSubR}
%
%\def\AXFalseESubL{false[\vec e/ Es]}
%\def\AXFalseESubR{false}
%\def\AXFalseESubN{\LNAME{Ax-$false$-ESubst}}
%\def\AXFalseESub{\AXFalseESubL \equiv \AXFalseESubR}
%
%\def\AXFalsePSubL{false[\vec q/ Ps]}
%\def\AXFalsePSubR{false}
%\def\AXFalsePSubN{\LNAME{Ax-$false$-PSubst}}
%\def\AXFalsePSub{\AXFalsePSubL \equiv \AXFalsePSubR}

\newpage
\verb"$$\AXNONPROP$$"
$$\AXNONPROP$$


\newpage
\verb"$$\INFERENCES$$"
$$\INFERENCES$$

\verb"$$\DEDUCTION$$"
$$\DEDUCTION$$

\newpage
\verb"$$\DERIVED$$"
$$\DERIVED$$

